removing wpd

theories/lang/cpp/logic/destructors.v
@@ -1,53 +1,202 @@
 (*
- * Copyright (C) BedRock Systems Inc. 2019-2020 Gregory Malecha
+ * Copyright (C) BedRock Systems Inc. 2019 Gregory Malecha
  *
  * SPDX-License-Identifier: LGPL-2.1 WITH BedRock Exception for use over network, see repository root for details.
  *)
-Require Import Coq.Lists.List.
-
-From bedrock.lang.cpp Require Import ast semantics.
+Require Import Coq.ZArith.ZArith.
+Require Import bedrock.lang.cpp.ast.
+Require Import bedrock.lang.cpp.semantics.
 From bedrock.lang.cpp.logic Require Import
-     pred path_pred heap_pred wp destroy.
+     pred wp path_pred heap_pred.
+Require Import bedrock.lang.cpp.logic.dispatch.
 
-Section with_resolve.
-  Context `{Σ : cpp_logic thread_info} {σ: genv}.
-  Variables (M : coPset) (ti : thread_info) (ρ : region).
+Require Import bedrock.lang.cpp.heap_notations.
 
-  Definition type_of_field (cls : globname) (f : ident) : option type :=
-    match σ.(genv_tu) !! cls with
-    | None => None
-    | Some (Gstruct st) =>
-      match List.find (fun '(x,_,_,_) => bool_decide (f = x)) st.(s_fields) with
-      | Some (_, ty, _, _) => Some ty
-      | _ => None
+Set Default Proof Using "Type".
+
+Section destroy.
+  Context `{Σ : cpp_logic thread_info} {σ:genv}.
+  Variable (ti : thread_info).
+
+  Local Notation _sub := (_sub (resolve:=σ)) (only parsing).
+  Local Notation anyR := (anyR (resolve:=σ)) (only parsing).
+  Local Notation _global := (_global (resolve:=σ)) (only parsing).
+
+  (* TODO: move? *)
+  Instance fold_left_ne {T : ofeT} {U : Type} {n} :
+    Proper ((dist n ==> pointwise_relation _ (dist n)) ==> eq ==> dist n ==> dist n) (@fold_left T U).
+  Proof.
+    do 4 red; intros f1 f2 Hf xs1 _ <-.
+    induction xs1; simpl; first done.
+    intros x1 x2 Hx.
+    eapply IHxs1, Hf, Hx.
+  Qed.
+
+  Fixpoint all_identities' (f : nat) (mdc : option globname) (cls : globname) : Rep :=
+    match f with
+    | 0 => lfalse
+    | S f =>
+      match σ.(genv_tu).(globals) !! cls with
+      | Some (Gstruct st) =>
+        _identity σ cls mdc 1 **
+        [∗list] b ∈ st.(s_bases),
+           let '(base,_) := b in
+           _base σ cls base |-> all_identities' f mdc base
+      | _ => False
       end
-    | _ => None
-    end.
+    end%I.
 
-  Definition get_type_of_path (from : globname) (p : FieldOrBase) : option type :=
-    match p with
-    | This => Some (Tnamed from)
-    | Field fn => type_of_field from fn
-    | Base gn => Some (Tnamed gn)
-    | Indirect ls i =>
-      (* this is a little bit awkward because we assume the correctness of
-         the type annotations in the path
-       *)
-      (fix go (from : globname) (ls : _) : option type :=
-         match ls with
-         | nil => type_of_field from i
-         | (_, gn) :: ls => go gn ls
-         end) from ls
-    end.
+  Definition all_identities : option globname -> globname -> Rep :=
+    let size := avl.IM.cardinal σ.(genv_tu).(globals) in
+    (* ^ the number of global entries is an upper bound on the height of the
+       derivation tree.
+     *)
+    all_identities' size.
 
-  Axiom wpd_deinit : forall (cls : globname) (this : val) path (Q : epred),
-    Exists fp,
-      (_offsetL (offset_for σ cls path) (_eqv this) &~ fp ** ltrue) //\\
-      (match get_type_of_path cls path with
-       | Some target_type =>
-         destruct_val (σ:=σ) ti target_type (Vptr fp) Q
-       | _ => lfalse
-       end)
-    |-- wpd (resolve:=σ) M ti ρ cls this path Q.
+  (** [revert_identities cls Q] destroys the identity of [cls] that lives at [this].
+      In doing so, it updates the identities of all base classes to have each base
+      be its own "most-derived-class".
 
-End with_resolve.
+      This is necessary to make virtual dispatch work correctly when base classes
+      are destroyed.
+   *)
+  Definition revert_identity (cls : globname) (Q : mpred) : Rep :=
+    match σ.(genv_tu).(globals) !! cls with
+    | Some (Gstruct st) =>
+      _identity σ cls (Some cls) 1 **
+      ([∗list] b ∈ st.(s_bases),
+          let '(base,_) := b in
+          _base σ cls base |-> all_identities (Some cls) base) **
+      (_identity σ cls None 1 -*
+       ([∗list] b ∈ st.(s_bases),
+         let '(base,_) := b in
+         _base σ cls base |-> all_identities (Some base) base) -* pureR Q)
+    | _ => False
+    end%I.
+
+  Instance revert_identity_ne : Proper (dist n ==> dist n) (revert_identity cls).
+  Proof.
+    red. red. rewrite /revert_identity; intros.
+    repeat case_match =>//.
+    solve_proper.
+  Qed.
+
+  Unset Program Cases.
+
+  Program Definition wp_default_dtor_pre (destruct_type : type -d> Loc -d> mpredI -n> mpredI)
+    : globname -d> Struct -d> Loc -d> mpredI -n> mpredI :=
+    λ cls st this, λne Q,
+    let bases :=
+        fold_left (fun Q '(base, _) =>
+                     |> destruct_type (Tnamed base) (_offsetL (_base σ cls base) this) Q) st.(s_bases) Q
+    in
+    let ident := this |-> revert_identity cls bases in
+    fold_left (fun Q '(x,ty,_,_) =>
+                 match drop_qualifiers ty with
+                 | Tnamed nm =>
+                   let l' := _offsetL (_field (resolve:=σ) {| f_type := cls ; f_name := x |}) this  in
+                   |> destruct_type ty l' Q
+                 | _ => Q
+                 end) st.(s_fields) ident.
+  Next Obligation.
+    intros ? ? ? ? ? ? ? ?; simpl.
+    apply fold_left_ne; eauto.
+    { intros ? ? ? ?; repeat case_match =>/=; eauto.
+      rewrite H0. reflexivity. }
+    { apply _at_ne. apply revert_identity_ne.
+      apply fold_left_ne; try done.
+      do 4 intro; repeat case_match => //; subst; f_contractive.
+      apply ofe_mor_car_ne, dist_S; eauto. }
+  Qed.
+
+  Instance wp_default_dtor_contractive : Contractive wp_default_dtor_pre.
+  Proof.
+    intros n f1 f2 Hf cls st this Q.
+    unfold wp_default_dtor_pre; simpl.
+    apply fold_left_ne; eauto.
+    { intros ? ? ? ?; repeat case_match => /=; eauto.
+      rewrite H.
+      f_contractive. eapply Hf. }
+    apply _at_ne. apply revert_identity_ne.
+    apply fold_left_ne; try done.
+    do 4 intro; repeat case_match => /=. rewrite H. f_contractive. apply Hf.
+  Qed.
+
+  Program Definition wp_dtor_pre (destruct_type : type -d> Loc -d> mpredI -n> mpredI)
+    : type -d> Loc -d> mpredI -n> mpredI :=
+    λ t this, λne Q,
+       match drop_qualifiers t with
+       | Tnamed cls =>
+         match σ.(genv_tu).(globals) !! cls with
+         | Some (Gstruct st) =>
+           match st.(s_dtor) with
+           | DtorDeleted => False
+           | DtorUser nm =>
+             match σ.(genv_tu).(symbols) !! nm with
+             | Some (Odestructor d) =>
+               let dt := type_of_value (Odestructor d) in
+              Exists da thisp, _global nm &~ da ** this &~ thisp **
+                                        |> fspec σ.(genv_tu).(globals) dt ti (Vptr da) (Vptr thisp :: nil) (fun _ => Q)
+             | _ => False
+             end
+           | DtorDefault =>
+             wp_default_dtor_pre destruct_type cls st this Q
+           end
+         | Some (Gunion _) => Q
+         | Some (Genum t _) => |> destruct_type t this Q
+         | _ => False
+         end
+       | Tarray ty n =>
+         (* destroy an array by destroying each element starting from the end *)
+         List.fold_left (fun Q off =>
+                           |> destruct_type ty (this ., (_sub ty (Z.of_nat off))) Q) (seq 0 (N.to_nat n)) Q
+       | Tptr _ | Tref _ | Trv_ref _
+       | Tint _ _ | Tfunction _ _ | Tbool | Tmember_pointer _ _ | Tfloat _
+       | Tnullptr | Tarch _ _ => Q
+
+       | Tqualified _ _ | Tvoid => False
+       end%I.
+  Next Obligation.
+    intros wp_dtor t this n Q1 Q2 HQ.
+    simpl.
+    repeat case_match; try fast_done; first last. {
+      f_contractive.
+      by apply ofe_mor_car_ne, dist_S, HQ.
+    }
+    by repeat f_equiv.
+    apply wp_default_dtor_pre; eauto.
+    apply fold_left_ne; try done.
+    do 4 intro. rewrite H. eauto.
+  Qed.
+
+  Instance wp_dtor_pre_contractive : Contractive wp_dtor_pre.
+  Proof.
+    intros n f1 f2 Hf t this Q.
+    unfold wp_dtor_pre; simpl.
+    repeat case_match; try fast_done; first last. {
+      f_contractive.
+      apply Hf.
+    }
+    eapply wp_default_dtor_contractive; eauto.
+    apply fold_left_ne; try done.
+    do 4 intro. rewrite H. f_contractive. apply Hf.
+  Qed.
+
+  (** [wp_dtor ty this Q] represents the weakest pre-condition for invoking the
+      destructor for the type [ty] on the location [this] with post-condition [Q].
+
+      Note that this is like the weakest pre-condition for a function, it does
+      perform virtual dispatch.
+   *)
+  Definition wp_dtor : type -d> Loc -d> mpredI -n> mpredI :=
+    fixpoint wp_dtor_pre.
+
+  Lemma wp_dtor_unfold : wp_dtor ≡ wp_dtor_pre wp_dtor.
+  Proof. apply fixpoint_unfold. Qed.
+
+  Lemma wp_dtor_unfold_eta t this Q : wp_dtor t this Q ≡ wp_dtor_pre wp_dtor t this Q.
+  Proof. apply wp_dtor_unfold. Qed.
+
+  Definition wp_default_dtor := wp_default_dtor_pre wp_dtor.
+
+End destroy.
